thys-2019/lib/Bits_Natural.thy
@@ -1,0 +1,259 @@
+(* Author: Mathias Fleury
+   Minor additions by Peter Lammich
+*)
+theory Bits_Natural
+  imports "HOL-Word.Word"
+begin
+
+(* TODO: Move *)
+lemma bin_trunc_xor':
+  "bintrunc n x XOR bintrunc n y = bintrunc n (x XOR y)"
+  by (auto simp add: bin_eq_iff bin_nth_ops nth_bintr)
+
+lemma uint_xor: "uint (x XOR y) = uint x XOR uint y"
+  by (transfer, simp add: bin_trunc_xor')
+
+
+
+instantiation nat :: bit_comprehension
+begin
+
+definition test_bit_nat :: \<open>nat \<Rightarrow> nat \<Rightarrow> bool\<close> where
+  "test_bit i j = test_bit (int i) j"
+
+definition lsb_nat :: \<open>nat \<Rightarrow> bool\<close> where
+  "lsb i = (int i :: int) !! 0"
+
+definition set_bit_nat :: "nat \<Rightarrow> nat \<Rightarrow> bool \<Rightarrow> nat" where
+  "set_bit i n b = nat (bin_sc n b (int i))"
+
+definition set_bits_nat :: "(nat \<Rightarrow> bool) \<Rightarrow> nat" where
+  "set_bits f =
+  (if \<exists>n. \<forall>n'\<ge>n. \<not> f n' then
+     let n = LEAST n. \<forall>n'\<ge>n. \<not> f n'
+     in nat (bl_to_bin (rev (map f [0..<n])))
+   else if \<exists>n. \<forall>n'\<ge>n. f n' then
+     let n = LEAST n. \<forall>n'\<ge>n. f n'
+     in nat (sbintrunc n (bl_to_bin (True # rev (map f [0..<n]))))
+   else 0 :: nat)"
+
+definition shiftl_nat where
+  "shiftl x n = nat ((int x) * 2 ^ n)"
+
+definition shiftr_nat where
+  "shiftr x n = nat (int x div 2 ^ n)"
+
+definition bitNOT_nat :: "nat \<Rightarrow> nat" where
+  "bitNOT i = nat (bitNOT (int i))"
+
+definition bitAND_nat :: "nat \<Rightarrow> nat \<Rightarrow> nat" where
+  "bitAND i j = nat (bitAND (int i) (int j))"
+
+definition bitOR_nat :: "nat \<Rightarrow> nat \<Rightarrow> nat" where
+  "bitOR i j = nat (bitOR (int i) (int j))"
+
+definition bitXOR_nat :: "nat \<Rightarrow> nat \<Rightarrow> nat" where
+  "bitXOR i j = nat (bitXOR (int i) (int j))"
+
+instance ..
+
+end
+
+
+lemma nat_shiftr[simp]:
+  "m >> 0 = m"
+  \<open>((0::nat) >> m) = 0\<close>
+  \<open>(m >> Suc n) = (m div 2 >> n)\<close> for m :: nat
+  by (auto simp: shiftr_nat_def zdiv_int zdiv_zmult2_eq[symmetric])
+
+lemma nat_shifl_div: \<open>m >> n = m div (2^n)\<close> for m :: nat
+  by (induction n arbitrary: m) (auto simp: div_mult2_eq)
+
+lemma nat_shiftl[simp]:
+  "m << 0 = m"
+  \<open>((0::nat) << m) = 0\<close>
+  \<open>(m << Suc n) = ((m * 2) << n)\<close> for m :: nat
+  by (auto simp: shiftl_nat_def zdiv_int zdiv_zmult2_eq[symmetric])
+
+lemma nat_shiftr_div2: \<open>m >> 1 = m div 2\<close> for m :: nat
+  by auto
+
+lemma nat_shiftr_div: \<open>m << n = m * (2^n)\<close> for m :: nat
+  by (induction n arbitrary: m) (auto simp: div_mult2_eq)
+
+definition shiftl1 :: \<open>nat \<Rightarrow> nat\<close> where
+  \<open>shiftl1 n = n << 1\<close>
+
+definition shiftr1 :: \<open>nat \<Rightarrow> nat\<close> where
+  \<open>shiftr1 n = n >> 1\<close>
+
+instantiation natural :: bit_comprehension
+begin
+
+context includes natural.lifting begin
+
+lift_definition test_bit_natural :: \<open>natural \<Rightarrow> nat \<Rightarrow> bool\<close> is test_bit .
+
+lift_definition lsb_natural :: \<open>natural \<Rightarrow> bool\<close> is lsb .
+
+lift_definition set_bit_natural :: "natural \<Rightarrow> nat \<Rightarrow> bool \<Rightarrow> natural" is
+  set_bit .
+
+lift_definition set_bits_natural :: \<open>(nat \<Rightarrow> bool) \<Rightarrow> natural\<close>
+  is \<open>set_bits :: (nat \<Rightarrow> bool) \<Rightarrow> nat\<close> .
+
+lift_definition shiftl_natural :: \<open>natural \<Rightarrow> nat \<Rightarrow> natural\<close>
+  is \<open>shiftl :: nat \<Rightarrow> nat \<Rightarrow> nat\<close> .
+
+lift_definition shiftr_natural :: \<open>natural \<Rightarrow> nat \<Rightarrow> natural\<close>
+  is \<open>shiftr :: nat \<Rightarrow> nat \<Rightarrow> nat\<close> .
+
+lift_definition bitNOT_natural :: \<open>natural \<Rightarrow> natural\<close>
+  is \<open>bitNOT :: nat \<Rightarrow> nat\<close> .
+
+lift_definition bitAND_natural :: \<open>natural \<Rightarrow> natural \<Rightarrow> natural\<close>
+  is \<open>bitAND :: nat \<Rightarrow> nat \<Rightarrow> nat\<close> .
+
+lift_definition bitOR_natural :: \<open>natural \<Rightarrow> natural \<Rightarrow> natural\<close>
+  is \<open>bitOR :: nat \<Rightarrow> nat \<Rightarrow> nat\<close> .
+
+lift_definition bitXOR_natural :: \<open>natural \<Rightarrow> natural \<Rightarrow> natural\<close>
+  is \<open>bitXOR :: nat \<Rightarrow> nat \<Rightarrow> nat\<close> .
+
+end
+
+instance ..
+end
+
+
+lemma bitXOR_1_if_mod_2: \<open>bitXOR L 1 = (if L mod 2 = 0 then L + 1 else L - 1)\<close> for L :: nat
+  apply transfer
+  apply (subst int_int_eq[symmetric])
+  apply (rule bin_rl_eqI)
+   apply (auto simp: bitXOR_nat_def)
+  unfolding bin_rest_def bin_last_def bitXOR_nat_def
+       apply presburger+
+  done
+
+lemma bitAND_1_mod_2: \<open>bitAND L 1 = L mod 2\<close> for L :: nat
+  apply transfer
+  apply (subst int_int_eq[symmetric])
+  apply (subst bitAND_nat_def)
+  by (auto simp: zmod_int bin_rest_def bin_last_def bitval_bin_last[symmetric])
+
+
+lemma nat_set_bit_0: \<open>set_bit x 0 b = nat ((bin_rest (int x)) BIT b)\<close> for x :: nat
+  by (auto simp: set_bit_nat_def)
+
+lemma nat_test_bit0_iff: \<open>n !! 0 \<longleftrightarrow> n mod 2 = 1\<close> for n :: nat
+proof -
+  have 2: \<open>2 = int 2\<close>
+    by auto
+  have [simp]: \<open>int n mod 2 = 1 \<longleftrightarrow> n mod 2 = Suc 0\<close>
+    unfolding 2 zmod_int[symmetric]
+    by auto
+
+  show ?thesis
+    unfolding test_bit_nat_def
+    by (auto simp: bin_last_def zmod_int)
+qed
+lemma test_bit_2: \<open>m > 0 \<Longrightarrow> (2*n) !! m \<longleftrightarrow> n !! (m - 1)\<close> for n :: nat
+  by (cases m)
+    (auto simp: test_bit_nat_def bin_rest_def)
+
+lemma test_bit_Suc_2: \<open>m > 0 \<Longrightarrow> Suc (2 * n) !! m \<longleftrightarrow> (2 * n) !! m\<close> for n :: nat
+  by (cases m)
+    (auto simp: test_bit_nat_def bin_rest_def)
+
+lemma bin_rest_prev_eq:
+  assumes [simp]: \<open>m > 0\<close>
+  shows  \<open>nat ((bin_rest (int w))) !! (m - Suc (0::nat)) = w !! m\<close>
+proof -
+  define m' where \<open>m' = w div 2\<close>
+  have w: \<open>w = 2 * m' \<or> w = Suc (2 * m')\<close>
+    unfolding m'_def
+    by auto
+  moreover have \<open>bin_nth (int m') (m - Suc 0) = m' !! (m - Suc 0)\<close>
+    unfolding test_bit_nat_def test_bit_int_def ..
+  ultimately show ?thesis
+    by (auto simp: bin_rest_def test_bit_2 test_bit_Suc_2)
+qed
+
+lemma bin_sc_ge0: \<open>w >= 0 ==> (0::int) \<le> bin_sc n b w\<close>
+  by (induction n arbitrary: w) auto
+
+lemma bin_to_bl_eq_nat:
+  \<open>bin_to_bl (size a) (int a) = bin_to_bl (size b) (int b) ==> a=b\<close>
+  by (metis Nat.size_nat_def size_bin_to_bl)
+
+lemma nat_bin_nth_bl: "n < m \<Longrightarrow> w !! n = nth (rev (bin_to_bl m (int w))) n" for w :: nat
+  apply (induct n arbitrary: m w)
+  subgoal for m w
+    apply clarsimp
+    apply (case_tac m, clarsimp)
+    using bin_nth_bl bin_to_bl_def test_bit_int_def test_bit_nat_def apply presburger
+    done
+  subgoal for n m w
+    apply (clarsimp simp: bin_to_bl_def)
+    apply (case_tac m, clarsimp)
+    apply (clarsimp simp: bin_to_bl_def)
+    apply (subst bin_to_bl_aux_alt)
+    apply (simp add: bin_nth_bl test_bit_nat_def)
+    done
+  done
+
+lemma bin_nth_ge_size: \<open>nat na \<le> n \<Longrightarrow> 0 \<le> na \<Longrightarrow> bin_nth na n = False\<close>
+proof (induction \<open>n\<close> arbitrary: na)
+  case 0
+  then show ?case by auto
+next
+  case (Suc n na) note IH = this(1) and H = this(2-)
+  have \<open>na = 1 \<or> 0 \<le> na div 2\<close>
+    using H by auto
+  moreover have
+    \<open>na = 0 \<or> na = 1 \<or> nat (na div 2) \<le> n\<close>
+    using H by auto
+  ultimately show ?case
+    using IH[rule_format,  of \<open>bin_rest na\<close>] H
+    by (auto simp: bin_rest_def)
+qed
+
+lemma test_bit_nat_outside: "n > size w \<Longrightarrow> \<not>w !! n" for w :: nat
+  unfolding test_bit_nat_def
+  by (auto simp: bin_nth_ge_size)
+
+lemma nat_bin_nth_bl':
+  \<open>a !! n \<longleftrightarrow> (n < size a \<and> (rev (bin_to_bl (size a) (int a)) ! n))\<close>
+  by (metis (full_types) Nat.size_nat_def bin_nth_ge_size leI nat_bin_nth_bl nat_int
+      of_nat_less_0_iff test_bit_int_def test_bit_nat_def)
+
+lemma nat_set_bit_test_bit: \<open>set_bit w n x !! m = (if m = n then x else w !! m)\<close> for w n :: nat
+  unfolding nat_bin_nth_bl'
+  apply auto
+        apply (metis bin_nth_bl bin_nth_sc bin_nth_simps(3) bin_to_bl_def int_nat_eq set_bit_nat_def)
+       apply (metis bin_nth_ge_size bin_nth_sc bin_sc_ge0 leI of_nat_less_0_iff set_bit_nat_def)
+      apply (metis bin_nth_bl bin_nth_ge_size bin_nth_sc bin_sc_ge0 bin_to_bl_def int_nat_eq leI
+      of_nat_less_0_iff set_bit_nat_def)
+     apply (metis Nat.size_nat_def bin_nth_sc_gen bin_nth_simps(3) bin_to_bl_def int_nat_eq
+      nat_bin_nth_bl' set_bit_nat_def test_bit_int_def test_bit_nat_def)
+    apply (metis Nat.size_nat_def bin_nth_bl bin_nth_sc_gen bin_to_bl_def int_nat_eq nat_bin_nth_bl
+      nat_bin_nth_bl' of_nat_less_0_iff of_nat_less_iff set_bit_nat_def)
+   apply (metis (full_types) bin_nth_bl bin_nth_ge_size bin_nth_sc_gen bin_sc_ge0 bin_to_bl_def leI of_nat_less_0_iff set_bit_nat_def)
+  by (metis bin_nth_bl bin_nth_ge_size bin_nth_sc_gen bin_sc_ge0 bin_to_bl_def int_nat_eq leI of_nat_less_0_iff set_bit_nat_def)
+
+  
+  
+lemma unat_or: "unat (x OR y) = unat x OR unat y"
+  unfolding unat_def
+  by (simp add: uint_or bitOR_nat_def)
+
+lemma unat_and: "unat (x AND y) = unat x AND unat y"
+  unfolding unat_def
+  by (simp add: uint_and bitAND_nat_def)
+  
+lemma unat_xor: "unat (x XOR y) = unat x XOR unat y"
+  unfolding unat_def
+  by (simp add: uint_xor bitXOR_nat_def)
+  
+  
+end
