thys-2019/sepref/Sepref_Basic.thy
@@ -146,7 +146,7 @@ subsection \<open>Constraints in Refinement Relations\<close>
 definition rdomp :: "('a \<Rightarrow> 'c \<Rightarrow> assn) \<Rightarrow> 'a \<Rightarrow> bool" where
   "rdomp R a \<equiv> \<exists>h c. R a c h"
 
-abbreviation "rdom R \<equiv> Collect (rdomp R)"
+(*abbreviation "rdom R \<equiv> Collect (rdomp R)"*)
 
 lemma rdomp_ctxt[simp]: "rdomp (hn_ctxt R) = rdomp R"
   by (simp add: hn_ctxt_def[abs_def])  
@@ -154,8 +154,9 @@ lemma rdomp_ctxt[simp]: "rdomp (hn_ctxt R) = rdomp R"
 lemma rdomp_pure[simp]: "rdomp (pure R) a \<longleftrightarrow> a\<in>Range R"
   unfolding rdomp_def pure_def by (auto simp: pred_lift_extract_simps)
 
-lemma rdom_pure[simp]: "rdom (pure R) = Range R"
+(*lemma rdom_pure[simp]: "rdom (pure R) = Range R"
   unfolding rdomp_def[abs_def] pure_def by (auto simp: pred_lift_extract_simps)
+*)  
 
 lemma Range_of_constraint_conv[simp]: "Range (A\<inter>UNIV\<times>C) = Range A \<inter> C"
   by auto
